iris/PipesOut.v
@@ -51,8 +51,187 @@ From stdpp Require Import list.
 Local Open Scope list_scope.
 
 (* ===================================================================== *)
-(*  1.  THE SINGLE-WRITER STEPS, over any content function and admission *)
+(*  1.  THE SINGLE-WRITER STEPS, over any line model (cut C9c'), and at  *)
+(*      the pipeline application's                                       *)
 (* ===================================================================== *)
+Section pipes_writes_v.
+  Context {Σ : gFunctors}.
+  Context `{!echoOutG Σ, !pipeOutG Σ}.
+  Context (g : pipe_gn).
+  Context (M : lmodel) (G : gen_cparams M) (B : lm_byte_laws M) (sd : lm_st M).
+  Context (WA : gen_wa M G sd).
+  Local Notation T := (gcT G).
+  Local Notation PIN := (gcPIN G).
+  Local Notation PCV := (peclV g M G sd WA).
+
+  (* (W) THE WRITE INSIDE A BLOCK OR A PROLOGUE ROUND.  An open round has
+     already written its block's first byte, so the writer's byte -- one
+     the stream owes BEFORE the input's end -- cannot be the open round's
+     next one: the writer's input would have to be the whole echoed list,
+     which ends at the open round's line. *)
+  Lemma peclV_step_write (k : nat) (v : era_pins) (P : nat) (b : bv 8)
+      (ps0 cs0 : list nat) (s0 : lm_st M) (I0 : list (bv 8)) (ho : list mobs)
+      (H : LogEntryDefs.cons_hist) :
+    (nlines I0 <= length cs0)%nat ->
+    lm_pro_pin M ps0 cs0 I0 ->
+    lm_proc_stream M ps0 cs0 s0 I0 !! P = Some b ->
+    PIN k v -∗ turn v P -∗ ps_lb v ps0 -∗ cs_lb v cs0 -∗ inp_lb v I0 -∗ gcW G k s0 -∗
+    PCV k ho H ==∗
+      PCV k ho (ConsLog.cons_step H (ConsLog.EvOut b))
+      ∗ ((turn v (S P) ∗ ps_lb v ps0 ∗ cs_lb v cs0 ∗ inp_lb v I0 ∗ gcW G k s0) ∨ T).
+  Proof using .
+    intros Hn Hpin0 Hb.
+    iIntros "#Hpin Ht #Hpslb #Hcslb #Hilb #HW Hcl". rewrite !peclV_gen.
+    iDestruct "Hcl" as "[Hc | Hp]".
+    - iMod (gcl_step_write M G sd WA k v P b ps0 cs0 s0 I0 ho H Hn Hpin0 Hb
+              with "Hpin Ht Hpslb Hcslb Hilb HW Hc") as "[Hc Hr]".
+      iModIntro. iSplitL "Hc"; [by iLeft |].
+      iDestruct "Hr" as "[(Ht & Hps & Hcs & Hi & HW2) | HT]";
+        [iLeft; by iFrame | by iRight].
+    - iDestruct "Hp" as (v2 w so r gb pre tm)
+        "(#Hpin2 & #Hpera & Hwa & Hblk & Hcur & Hrb & Hta & Hcs & Hps & HE & Hdl & Hdll & %Hopen)".
+      iDestruct (gcPIN_agree G with "Hpin2 Hpin") as %->.
+      iDestruct (gwa_agree WA with "Hwa HW") as %Hst.
+      assert (Hst' : gs_state M sd so = s0) by exact Hst.
+      clear Hst. subst s0.
+      iDestruct (turn_agree with "Ht Hta") as %HP.
+      iDestruct (pcs_lb_prefix with "Hcs Hcslb") as %Hcsp.
+      iDestruct (ps_lb_prefix with "Hps Hpslb") as %Hpsp.
+      iDestruct (inp_lb_le with "Hdll Hilb") as %HI0dl.
+      assert (HI0 : I0 `prefix_of` (snd <$> gs_E M so)).
+      { etrans; [exact HI0dl | exact (gcl_pure_o_dl_E M sd _ _ _ _ _ _ Hopen)]. }
+      destruct (lm_write_stage_byte M ps0 (gs_ps M so) cs0 (gs_cs M so)
+                  (gs_state M sd so) (gs_E M so) (gs_w M so) I0 P b
+                  Hpsp Hpin0 Hcsp Hn HI0 HP Hb) as [HlenE _].
+      destruct Hopen as (_ & Hop & _).
+      destruct (lm_blk_open_cs M sd so r pre Hop) as (Hq & Hrr & Hnn).
+      pose proof (prefix_length _ _ Hcsp) as Hcl0.
+      rewrite HlenE in Hq, Hrr, Hnn.
+      pose proof (nlines_pos_of_rest_nil I0 Hnn Hrr) as Hpos0.
+      exfalso. lia.
+  Qed.
+
+  (* (W') THE WRITE AT A BLOCK'S FIRST BYTE, which FILES the alternative:
+     a single-writer round (an echo line's).  An open round has already
+     written a byte of the block this writer would open. *)
+  Lemma peclV_step_write_blk (k : nat) (v : era_pins) (P a : nat) (b : bv 8)
+      (ps0 cs0 : list nat) (s0 : lm_st M) (I0 : list (bv 8)) (ho : list mobs)
+      (H : LogEntryDefs.cons_hist) :
+    I0 <> [] ->
+    rest_of I0 = [] ->
+    (nlines I0 <= S (length cs0))%nat ->
+    lm_pro_pin M ps0 cs0 I0 ->
+    P = length (lm_proc_before M ps0 cs0 s0 I0) ->
+    lm_ok M (lm_upto M cs0 s0 (bodies_of I0) (nlines I0 - 1))
+      (lm_of M (bodies_of I0 !!! (nlines I0 - 1)%nat)) (lm_dec M a) ->
+    lm_term M (lm_dec M a) = false ->
+    lm_cont M (lm_upto M cs0 s0 (bodies_of I0) (nlines I0 - 1))
+      (lm_of M (bodies_of I0 !!! (nlines I0 - 1)%nat)) (lm_dec M a) !! 0%nat = Some b ->
+    PIN k v -∗ turn v P -∗ ps_lb v ps0 -∗ cs_lb v cs0 -∗ inp_lb v I0 -∗ gcW G k s0 -∗
+    PCV k ho H ==∗
+      PCV k ho (ConsLog.cons_step H (ConsLog.EvOut b))
+      ∗ ((turn v (S P) ∗ ps_lb v ps0 ∗ cs_lb v (cs0 ++ [a]) ∗ inp_lb v I0 ∗ gcW G k s0) ∨ T).
+  Proof using B.
+    intros Hne0 Hr0 Hdiv Hpin0 HPeq Hok Hterm Hhead.
+    iIntros "#Hpin Ht #Hpslb #Hcslb #Hilb #HW Hcl". rewrite !peclV_gen.
+    iDestruct "Hcl" as "[Hc | Hp]".
+    - iMod (gcl_step_write_blk M G B sd WA k v P a b ps0 cs0 s0 I0 ho H
+              Hne0 Hr0 Hdiv Hpin0 HPeq Hok Hterm Hhead
+              with "Hpin Ht Hpslb Hcslb Hilb HW Hc") as "[Hc Hr]".
+      iModIntro. iSplitL "Hc"; [by iLeft |].
+      iDestruct "Hr" as "[(Ht & Hps & Hcs & Hi & HW2) | HT]";
+        [iLeft; by iFrame | by iRight].
+    - iDestruct "Hp" as (v2 w so r gb pre tm)
+        "(#Hpin2 & #Hpera & Hwa & Hblk & Hcur & Hrb & Hta & Hcs & Hps & HE & Hdl & Hdll & %Hopen)".
+      iDestruct (gcPIN_agree G with "Hpin2 Hpin") as %->.
+      iDestruct (gwa_agree WA with "Hwa HW") as %Hst.
+      assert (Hst' : gs_state M sd so = s0) by exact Hst.
+      clear Hst. subst s0.
+      iDestruct (turn_agree with "Ht Hta") as %HP.
+      iDestruct (pcs_lb_prefix with "Hcs Hcslb") as %Hcsp.
+      iDestruct (ps_lb_prefix with "Hps Hpslb") as %Hpsp.
+      iDestruct (inp_lb_le with "Hdll Hilb") as %HI0dl.
+      assert (HI0 : I0 `prefix_of` (snd <$> gs_E M so)).
+      { etrans; [exact HI0dl | exact (gcl_pure_o_dl_E M sd _ _ _ _ _ _ Hopen)]. }
+      destruct Hopen as (_ & Hop & _).
+      pose proof Hop as (_ & Hwpre' & Hne' & _).
+      assert (Hs2 : lm_proc_before M ps0 cs0 (gs_state M sd so) I0
+                    = lm_proc_before M (gs_ps M so) (gs_cs M so) (gs_state M sd so) I0).
+      { apply (lm_proc_before_cs_prefix M ps0 (gs_ps M so) cs0 (gs_cs M so) (gs_state M sd so) I0
+                 Hpsp Hcsp Hpin0).
+        rewrite (ll_nlines_removelast I0 Hr0). lia. }
+      pose proof (prefix_length _ _
+        (lm_proc_before_prefix M (gs_ps M so) (gs_cs M so) (gs_state M sd so) I0
+           (snd <$> gs_E M so) HI0)) as Hle2.
+      assert (Hwne : (1 <= length (gs_w M so))%nat).
+      { rewrite Hwpre'. destruct pre; [by destruct (Hne' eq_refl) | cbn; lia]. }
+      rewrite /lm_pcount in HP. rewrite HPeq Hs2 in HP.
+      exfalso. lia.
+  Qed.
+
+  (* (W-pro) THE WRITE AT A PROLOGUE ROUND'S CHOICE BYTE.  It comes after
+     the whole stream through [I0], which an open round's own bytes run
+     past already. *)
+  Lemma peclV_step_write_pro (k : nat) (v : era_pins) (P a : nat) (b : bv 8)
+      (ps0 cs0 : list nat) (s0 : lm_st M) (I0 : list (bv 8)) (ho : list mobs)
+      (CH : LogEntryDefs.cons_hist) :
+    0 < P \/ gwa_strict WA \/ gwa_free WA ->
+    rest_of I0 = [] ->
+    (I0 = [] \/ lm_panic M (lm_at M cs0 (nlines I0 - 1)%nat) = true) ->
+    (nlines I0 <= length cs0)%nat ->
+    lm_pro_pin M ps0 cs0 I0 ->
+    ~ pro_done (pro_from (lm_pro_idx M cs0 (nlines I0)) ps0) ->
+    P = length (lm_proc_stream M ps0 cs0 s0 I0) ->
+    (a < length pro_alts)%nat ->
+    pro_alts !!! a !! 0%nat = Some b ->
+    PIN k v -∗ turn v P -∗ ps_lb v ps0 -∗ cs_lb v cs0 -∗ inp_lb v I0 -∗ gcW G k s0 -∗
+    PCV k ho CH ==∗
+      PCV k ho (ConsLog.cons_step CH (ConsLog.EvOut b))
+      ∗ ((turn v (S P) ∗ ps_lb v (ps0 ++ [a]) ∗ cs_lb v cs0 ∗ inp_lb v I0 ∗ gcW G k s0) ∨ T).
+  Proof using .
+    intros HP0 Hr0 Hopen Hdiv Hpin0 Hnd HPeq Halt Hhead.
+    iIntros "#Hpin Ht #Hpslb #Hcslb #Hilb #HW Hcl". rewrite !peclV_gen.
+    iDestruct "Hcl" as "[Hc | Hp]".
+    - iMod (gcl_step_write_pro M G sd WA k v P a b ps0 cs0 s0 I0 ho CH
+              HP0 Hr0 Hopen Hdiv Hpin0 Hnd HPeq Halt Hhead
+              with "Hpin Ht Hpslb Hcslb Hilb HW Hc") as "[Hc Hr]".
+      iModIntro. iSplitL "Hc"; [by iLeft |].
+      iDestruct "Hr" as "[(Ht & Hps & Hcs & Hi & HW2) | HT]";
+        [iLeft; by iFrame | by iRight].
+    - iDestruct "Hp" as (v2 w so r gb pre tm)
+        "(#Hpin2 & #Hpera & Hwa & Hblk & Hcur & Hrb & Hta & Hcs & Hps & HE & Hdl & Hdll & %Hopen2)".
+      iDestruct (gcPIN_agree G with "Hpin2 Hpin") as %->.
+      iDestruct (gwa_agree WA with "Hwa HW") as %Hst.
+      assert (Hst' : gs_state M sd so = s0) by exact Hst.
+      clear Hst. subst s0.
+      iDestruct (turn_agree with "Ht Hta") as %HP.
+      iDestruct (pcs_lb_prefix with "Hcs Hcslb") as %Hcsp.
+      iDestruct (ps_lb_prefix with "Hps Hpslb") as %Hpsp.
+      iDestruct (inp_lb_le with "Hdll Hilb") as %HI0dl.
+      assert (HI0 : I0 `prefix_of` (snd <$> gs_E M so)).
+      { etrans; [exact HI0dl | exact (gcl_pure_o_dl_E M sd _ _ _ _ _ _ Hopen2)]. }
+      destruct Hopen2 as (_ & Hop & _).
+      pose proof Hop as (_ & Hwpre' & Hne' & _).
+      destruct (lm_blk_open_cs M sd so r pre Hop) as (Hqq & Hrr & Hne0').
+      assert (Hwne : (1 <= length (gs_w M so))%nat).
+      { rewrite Hwpre'. destruct pre; [by destruct (Hne' eq_refl) | cbn; lia]. }
+      rewrite /lm_pcount in HP.
+      destruct (decide ((snd <$> gs_E M so) = I0)) as [Heq | Hne2].
+      + rewrite Heq in Hqq, Hrr, Hne0'.
+        pose proof (nlines_pos_of_rest_nil I0 Hne0' Hrr) as Hpos0.
+        pose proof (prefix_length _ _ Hcsp) as Hcl0.
+        exfalso. lia.
+      + pose proof (lm_proc_stream_before M (gs_ps M so) (gs_cs M so) (gs_state M sd so) I0
+                      (snd <$> gs_E M so) HI0
+                      ltac:(intros Hq; apply Hne2; symmetry; exact Hq)) as Hpre2.
+        apply prefix_length in Hpre2.
+        pose proof (prefix_length _ _
+          (lm_proc_stream_prefix M ps0 (gs_ps M so) cs0 (gs_cs M so) (gs_state M sd so) I0
+             Hpsp Hcsp Hpin0 Hdiv)) as Hle3.
+        exfalso. lia.
+  Qed.
+End pipes_writes_v.
+
 Section pipes_writes.
   Context {Σ : gFunctors}.
   Context `{!echoOutG Σ, !pipeOutG Σ}.
@@ -86,34 +265,11 @@ Section pipes_writes.
       PC k ho (ConsLog.cons_step H (ConsLog.EvOut b))
       ∗ ((turn v (S P) ∗ ps_lb v ps0 ∗ cs_lb v cs0 ∗ inp_lb v I0) ∨ T).
   Proof using .
-    intros Hn Hpin0 Hb.
-    iIntros "#Hpin Ht #Hpslb #Hcslb #Hilb Hcl". rewrite !pecl'_gen.
-    iDestruct "Hcl" as "[Hc | Hp]".
-    - iAssert (gcW GP k tt) as "HW"; [done |].
-      iMod (gcl_step_write PM GP tt GA k v P b ps0 cs0 tt I0 ho H Hn Hpin0 Hb
-              with "Hpin Ht Hpslb Hcslb Hilb HW Hc") as "[Hc Hr]".
-      iModIntro. iSplitL "Hc"; [by iLeft |].
-      iDestruct "Hr" as "[(Ht & Hps & Hcs & Hi & _) | HT]";
-        [iLeft; by iFrame | by iRight].
-    - iDestruct "Hp" as (v2 w so r gb pre tm)
-        "(#Hpin2 & #Hpera & _ & Hblk & Hcur & Hrb & Hta & Hcs & Hps & HE & Hdl & Hdll & %Hopen)".
-      iDestruct (era_pin_agree with "Hpin2 Hpin") as %->.
-      iDestruct (turn_agree with "Ht Hta") as %HP.
-      iDestruct (pcs_lb_prefix with "Hcs Hcslb") as %Hcsp.
-      iDestruct (ps_lb_prefix with "Hps Hpslb") as %Hpsp.
-      iDestruct (inp_lb_le with "Hdll Hilb") as %HI0dl.
-      assert (HI0 : I0 `prefix_of` (snd <$> gs_E PM so)).
-      { etrans; [exact HI0dl | exact (gcl_pure_o_dl_E PM tt _ _ _ _ _ _ Hopen)]. }
-      rewrite -(pipes_st_tt so) in Hb.
-      destruct (lm_write_stage_byte PM ps0 (gs_ps PM so) cs0 (gs_cs PM so)
-                  (gs_state PM tt so) (gs_E PM so) (gs_w PM so) I0 P b
-                  Hpsp Hpin0 Hcsp Hn HI0 HP Hb) as [HlenE _].
-      destruct Hopen as (_ & Hop & _).
-      destruct (lm_blk_open_cs PM tt so r pre Hop) as (Hq & Hrr & Hnn).
-      pose proof (prefix_length _ _ Hcsp) as Hcl0.
-      rewrite HlenE in Hq, Hrr, Hnn.
-      pose proof (nlines_pos_of_rest_nil I0 Hnn Hrr) as Hpos0.
-      exfalso. lia.
+    intros Hn Hpin0 Hb. iIntros "Hpin Ht Hpslb Hcslb Hilb Hcl".
+    iMod (peclV_step_write g PM GP tt GA k v P b ps0 cs0 tt I0 ho H Hn Hpin0 Hb
+            with "Hpin Ht Hpslb Hcslb Hilb [] Hcl") as "[Hc Hr]"; [done |].
+    iModIntro. iSplitL "Hc"; [iExact "Hc" |].
+    iDestruct "Hr" as "[(Ht & Hps & Hcs & Hi & _) | HT]"; [iLeft; by iFrame | by iRight].
   Qed.
 
   (* (W') THE WRITE AT A BLOCK'S FIRST BYTE, which FILES the alternative:
@@ -137,39 +293,12 @@ Section pipes_writes.
       ∗ ((turn v (S P) ∗ ps_lb v ps0 ∗ cs_lb v (cs0 ++ [a]) ∗ inp_lb v I0) ∨ T).
   Proof using .
     intros Hne0 Hr0 Hdiv Hpin0 HPeq Hok Hterm Hhead.
-    iIntros "#Hpin Ht #Hpslb #Hcslb #Hilb Hcl". rewrite !pecl'_gen.
-    iDestruct "Hcl" as "[Hc | Hp]".
-    - iAssert (gcW GP k tt) as "HW"; [done |].
-      iMod (gcl_step_write_blk PM GP PB tt GA k v P a b ps0 cs0 tt I0 ho H
-              Hne0 Hr0 Hdiv Hpin0 HPeq Hok Hterm Hhead
-              with "Hpin Ht Hpslb Hcslb Hilb HW Hc") as "[Hc Hr]".
-      iModIntro. iSplitL "Hc"; [by iLeft |].
-      iDestruct "Hr" as "[(Ht & Hps & Hcs & Hi & _) | HT]";
-        [iLeft; by iFrame | by iRight].
-    - iDestruct "Hp" as (v2 w so r gb pre tm)
-        "(#Hpin2 & #Hpera & _ & Hblk & Hcur & Hrb & Hta & Hcs & Hps & HE & Hdl & Hdll & %Hopen)".
-      iDestruct (era_pin_agree with "Hpin2 Hpin") as %->.
-      iDestruct (turn_agree with "Ht Hta") as %HP.
-      iDestruct (pcs_lb_prefix with "Hcs Hcslb") as %Hcsp.
-      iDestruct (ps_lb_prefix with "Hps Hpslb") as %Hpsp.
-      iDestruct (inp_lb_le with "Hdll Hilb") as %HI0dl.
-      assert (HI0 : I0 `prefix_of` (snd <$> gs_E PM so)).
-      { etrans; [exact HI0dl | exact (gcl_pure_o_dl_E PM tt _ _ _ _ _ _ Hopen)]. }
-      destruct Hopen as (_ & Hop & _).
-      pose proof Hop as (_ & Hwpre' & Hne' & _).
-      rewrite (pipes_st_tt so) in HP.
-      assert (Hs2 : lm_proc_before PM ps0 cs0 tt I0
-                    = lm_proc_before PM (gs_ps PM so) (gs_cs PM so) tt I0).
-      { apply (lm_proc_before_cs_prefix PM ps0 (gs_ps PM so) cs0 (gs_cs PM so) tt I0
-                 Hpsp Hcsp Hpin0).
-        rewrite (ll_nlines_removelast I0 Hr0). lia. }
-      pose proof (prefix_length _ _
-        (lm_proc_before_prefix PM (gs_ps PM so) (gs_cs PM so) tt I0
-           (snd <$> gs_E PM so) HI0)) as Hle2.
-      assert (Hwne : (1 <= length (gs_w PM so))%nat).
-      { rewrite Hwpre'. destruct pre; [by destruct (Hne' eq_refl) | cbn; lia]. }
-      rewrite /lm_pcount in HP. rewrite HPeq Hs2 in HP.
-      exfalso. lia.
+    iIntros "Hpin Ht Hpslb Hcslb Hilb Hcl".
+    iMod (peclV_step_write_blk g PM GP PB tt GA k v P a b ps0 cs0 tt I0 ho H
+            Hne0 Hr0 Hdiv Hpin0 HPeq Hok Hterm Hhead
+            with "Hpin Ht Hpslb Hcslb Hilb [] Hcl") as "[Hc Hr]"; [done |].
+    iModIntro. iSplitL "Hc"; [iExact "Hc" |].
+    iDestruct "Hr" as "[(Ht & Hps & Hcs & Hi & _) | HT]"; [iLeft; by iFrame | by iRight].
   Qed.
 
   (* (W-pro) THE WRITE AT A PROLOGUE ROUND'S CHOICE BYTE.  It comes after
@@ -192,43 +321,12 @@ Section pipes_writes.
       ∗ ((turn v (S P) ∗ ps_lb v (ps0 ++ [a]) ∗ cs_lb v cs0 ∗ inp_lb v I0) ∨ T).
   Proof using .
     intros Hr0 Hopen Hdiv Hpin0 Hnd HPeq Halt Hhead.
-    iIntros "#Hpin Ht #Hpslb #Hcslb #Hilb Hcl". rewrite !pecl'_gen.
-    iDestruct "Hcl" as "[Hc | Hp]".
-    - iAssert (gcW GP k tt) as "HW"; [done |].
-      iMod (gcl_step_write_pro PM GP tt GA k v P a b ps0 cs0 tt I0 ho CH
-              (or_intror (or_intror I)) Hr0 Hopen Hdiv Hpin0 Hnd HPeq Halt Hhead
-              with "Hpin Ht Hpslb Hcslb Hilb HW Hc") as "[Hc Hr]".
-      iModIntro. iSplitL "Hc"; [by iLeft |].
-      iDestruct "Hr" as "[(Ht & Hps & Hcs & Hi & _) | HT]";
-        [iLeft; by iFrame | by iRight].
-    - iDestruct "Hp" as (v2 w so r gb pre tm)
-        "(#Hpin2 & #Hpera & _ & Hblk & Hcur & Hrb & Hta & Hcs & Hps & HE & Hdl & Hdll & %Hopen2)".
-      iDestruct (era_pin_agree with "Hpin2 Hpin") as %->.
-      iDestruct (turn_agree with "Ht Hta") as %HP.
-      iDestruct (pcs_lb_prefix with "Hcs Hcslb") as %Hcsp.
-      iDestruct (ps_lb_prefix with "Hps Hpslb") as %Hpsp.
-      iDestruct (inp_lb_le with "Hdll Hilb") as %HI0dl.
-      assert (HI0 : I0 `prefix_of` (snd <$> gs_E PM so)).
-      { etrans; [exact HI0dl | exact (gcl_pure_o_dl_E PM tt _ _ _ _ _ _ Hopen2)]. }
-      destruct Hopen2 as (_ & Hop & _).
-      pose proof Hop as (_ & Hwpre' & Hne' & _).
-      destruct (lm_blk_open_cs PM tt so r pre Hop) as (Hqq & Hrr & Hne0').
-      assert (Hwne : (1 <= length (gs_w PM so))%nat).
-      { rewrite Hwpre'. destruct pre; [by destruct (Hne' eq_refl) | cbn; lia]. }
-      rewrite (pipes_st_tt so) /lm_pcount in HP.
-      destruct (decide ((snd <$> gs_E PM so) = I0)) as [Heq | Hne2].
-      + rewrite Heq in Hqq, Hrr, Hne0'.
-        pose proof (nlines_pos_of_rest_nil I0 Hne0' Hrr) as Hpos0.
-        pose proof (prefix_length _ _ Hcsp) as Hcl0.
-        exfalso. lia.
-      + pose proof (lm_proc_stream_before PM (gs_ps PM so) (gs_cs PM so) tt I0
-                      (snd <$> gs_E PM so) HI0
-                      ltac:(intros Hq; apply Hne2; symmetry; exact Hq)) as Hpre2.
-        apply prefix_length in Hpre2.
-        pose proof (prefix_length _ _
-          (lm_proc_stream_prefix PM ps0 (gs_ps PM so) cs0 (gs_cs PM so) tt I0
-             Hpsp Hcsp Hpin0 Hdiv)) as Hle3.
-        exfalso. lia.
+    iIntros "Hpin Ht Hpslb Hcslb Hilb Hcl".
+    iMod (peclV_step_write_pro g PM GP tt GA k v P a b ps0 cs0 tt I0 ho CH
+            (or_intror (or_intror I)) Hr0 Hopen Hdiv Hpin0 Hnd HPeq Halt Hhead
+            with "Hpin Ht Hpslb Hcslb Hilb [] Hcl") as "[Hc Hr]"; [done |].
+    iModIntro. iSplitL "Hc"; [iExact "Hc" |].
+    iDestruct "Hr" as "[(Ht & Hps & Hcs & Hi & _) | HT]"; [iLeft; by iFrame | by iRight].
   Qed.
 End pipes_writes.
 
